\input{BASE-HEAD}
\newcommand{\laClass}       {CS 211}
\newcommand{\laSemester}    {Spring 2018}
\newcommand{\laChapter}     {5.5}
\newcommand{\laType}        {Exercise}
\newcommand{\laPoints}      {5}
\newcommand{\laTitle}       {Recursive Counting}
\newcommand{\laDate}        {Jan 16, 2018}
\setcounter{chapter}{5}
\setcounter{section}{5}
\addtocounter{section}{-1}
\newcounter{question}

\toggletrue{answerkey}

\input{BASE-HEADER}

\input{INSTRUCTIONS-EXERCISE}

    \begin{enumerate}
        \item[1a.]      First, check if $P(1,1) = 1$ works out. \\
                        $P(1,1) = 1 \cdot P( (1-1, 1-1) )$ \\
                        $ = 1 \cdot P( 0, 0 ) $ \tab
                        $ = 1 \cdot \frac{0!}{0!} $ \tab
                        $ = 1 \cdot \frac{1}{1} $ \tab
                        $ = 1 \cdot 1 $ \\
                        $ = 1 $ \checkmark \tab Checks out \\ 

                        Next, check for $P(n, 1) = n$... \\
                        $P(n, 1) = n \cdot P( (n-1), (1-1) )$ \\
                        $ = n \cdot P( n-1, 1 ) $ \tab
                        $ = n \cdot \frac{ (n-1)! }{ (n-1)! } $ \tab
                        $ = n \cdot 1 $ \\
                        $ = n $ \checkmark
                        
        \item[1b.]      $P(1,1)$ has been checked in part (a). \\

                        Check for $P(n,2) = n \cdot (n-1)$... \\
                        $P(n,2) = n \cdot P( (n-1), (2-1) )$ \\
                        $ = n \cdot \frac{ (n-1)! }{ (n-1-1)! } $ \tab
                        $ = n \cdot \frac{ (n-1)! }{ (n-2)! } $ \\
                        $ = n \cdot \frac{ (n-1) \cdot (n-2)! }{ (n-2)! } $ \tab
                        \small 
                        Expanded $(n-1)!$ in the numerator to $(n-1) \cdot (n-2)!$
                        \normalsize

                        $ = n \cdot (n-1)$ \checkmark 
                        
        \item[1c.]      $P(1,1)$ has been checked in part (a). \\

                        Check for $P(n,3) = n \cdot (n-1) \cdot (n-2)$... \\
                        $P(n,3) = n \cdot P( (n-1), (3-1) )$ \\
                        $ = n \cdot \frac{ (n-1)! }{ (n-1-2)! } $ \tab
                        $ = n \cdot \frac{ (n-1)! }{ (n-3)! } $ \tab Expand $(n-1)$ again... \\
                        $ = n \cdot \frac{ (n-1)(n-2)(n-3)! }{ (n-3)! } $ \\
                        $ = n \cdot (n-1) \cdot (n-2) $ \checkmark
    \end{enumerate}


\input{BASE-FOOT}
